Add a plugin to derive record setters using MetaCoq
This replaces the coq-record-update plugin based on Ltac that we used to
define nice record update syntax with a similarly one (on the surface)
that uses MetaCoq to define setters. The benefits are that we can
produce better terms and that we no longer have to list each member of
records when deriving. The downside is that it does not support indexed
records.

utils/theories/RecordSet.v
@@ -1,117 +1,129 @@
-(* Adapted from https://github.com/tchajed/coq-record-update; see NOTICE in the
-   root for license notice *)
+From MetaCoq.Template Require Import Ast.
+From MetaCoq.Template Require Import AstUtils.
+From MetaCoq.Template Require Import BasicAst.
+From MetaCoq.Template Require Import Loader.
+From MetaCoq.Template Require Import TemplateMonad.
+From MetaCoq.Template Require Import monad_utils.
+From MetaCoq.Template Require Import utils.
 
-Set Implicit Arguments.
+Global Unset Asymmetric Patterns.
 
-(** Reader is the reader monad (or just the function monad). We only use
-Applicative here. *)
-Definition Reader E T := forall (e:E), T e.
-Arguments Reader : clear implicits.
+Import MonadNotation.
 
-(* pure/return *)
-Definition constructor {E T} (x:T) : Reader E (fun _ => T) := fun _ => x.
+Class SetterFromGetter {A B} (a : A -> B) := setter_from_getter : (B -> B) -> A -> A.
 
-(* Always unfold constructor when applied with with a "final" argument. *)
-Arguments constructor {_ _} _ _ /.
+Definition aRelevant (na : name) : aname :=
+  {| binder_name := na; binder_relevance := Relevant |}.
 
-(* Applicative's (<*>) (written as `ap`).
+Definition make_setters (T : Type) : TemplateMonad unit :=
+  Tast <- tmQuote T;;
+  ind <- match Tast with
+        | tInd ind _ => ret ind
+        | tApp (tInd ind _) _ => ret ind
+        | _ => tmFail "Cannot extract inductive, are you sure you passed a type?"
+        end;;
+  mib <- tmQuoteInductive (inductive_mind ind);;
+  match ind_finite mib with
+  | BiFinite => ret tt
+  | _ => tmFail "Unexpected finite kind; are you sure you are creating setters for a record?"
+  end;;
+  oib <- match nth_error (ind_bodies mib) (inductive_ind ind) with
+         | Some oib => ret oib
+         | None => tmFail "Could not find inductive in mutual inductive?"
+         end;;
+  '(ctor, ar) <- match ind_ctors oib with
+                 | [((_, t), ar)] => ret (t, ar)
+                 | _ => tmFail "Type should have exactly one constructor"
+                 end;;
 
-This has an awkwardly long name since it's intended to be used infix with
- *)
-Definition applicative_ap {E}
-           {A: E -> Type}
-           {B: forall (e:E), A e -> Type}
-           (f: Reader E (fun e => forall (a:A e), B e a)) :
-  forall (x: Reader E A), Reader E (fun e => B e (x e))  :=
-  fun x => fun e => f e (x e).
+  let fix find_getter_kns (t : term) : TemplateMonad (list kername) :=
+      match t with
+      | tProd na A B =>
+        kn <-
+        match binder_name na with
+        | nNamed id => ret ((inductive_mind ind).1, id)
+        | nAnon => tmFail "Records with anonymous fields are not supported"
+        end;;
+        kns <- find_getter_kns B;;
+        ret (kn :: kns)
+      | tLetIn na a A B => find_getter_kns B
+      | _ => ret []
+      end in
 
-(** Settable is a way of accessing a constructor for a record of type T. The
-syntactic form of this definition is important: it must be an eta-expanded
-version of T's constructor, written generically over the field accessors of T.
-The best way to do this for a record X := mkX { A; B; C} is
-[settable! mkX <A; B; C>]. *)
-Class Settable T := { mkT: Reader T (fun _ => T);
-                      mkT_ok: forall x, mkT x = x }.
-Arguments mkT T mk : clear implicits, rename.
+  getter_kns <- find_getter_kns ctor;;
 
-Local Ltac solve_mkT_ok :=
-  match goal with
-  | |- forall x, _ = _ => solve [ destruct x; cbv; f_equal ]
-  end.
+  let fix create_setters (t : term) (idx : nat) : TemplateMonad unit :=
+      match t with
+      | tProd na A B =>
+        match binder_name na with
+        | nNamed id =>
+          (* Create setter *)
+          let getter_kn := ((inductive_mind ind).1, id) in
 
-(** settable! creates an instance of Settable from a constructor and list of
-fields. *)
-Notation "'settable!' mk < f1 ; .. ; fn >" :=
-  (Build_Settable
-     (applicative_ap .. (applicative_ap (constructor mk) f1) .. fn)
-     ltac:(solve_mkT_ok)) (at level 0, mk at level 10, f1, fn at level 9, only parsing).
+          let body :=
+              tLambda
+                (aRelevant (nNamed "f"))
+                (tProd (aRelevant nAnon) A A)
+                (tLambda
+                   (aRelevant (nNamed "r"))
+                   (tInd ind [])
+                   (tApp
+                      (tConstruct ind 0 [])
+                      (mapi
+                         (fun i (gkn : kername) =>
+                            let get := tApp (tConst gkn []) [tRel 0] in
+                            if eq_kername gkn getter_kn then
+                              tApp (tRel 1) [get]
+                            else
+                              get)
+                         getter_kns))) in
 
-(** [setter] creates a setter based on an eta-expanded record constructor and a
-particular field projection proj *)
-Local Ltac setter etaT proj :=
-  let set :=
-      (match eval pattern proj in etaT with
-       | ?setter ?proj => constr:(fun f => setter (fun r => f (proj r)))
-       end) in
-  let set := (eval cbv [constructor applicative_ap] in set) in
-  exact set.
+          let setter_id := "set_" ^ ind_name oib ^ "_" ^ id in
+          tmMkDefinition setter_id body;;
 
-(* Combining the above, [getSetter'] looks up the eta-expanded version of T with
-the Settable typeclass, and calls [setter] to create a setter. *)
-Local Ltac get_setter T proj :=
-  match constr:(mkT T _) with
-  | mkT _ ?updateable =>
-    let updateable := (eval hnf in updateable) in
-    match updateable with
-    | {| mkT := ?mk |} =>
-      setter mk proj
-    end
-  end.
+          (* Create SetterFromGetter instance *)
+          setter_gr <- tmLocate1 setter_id;;
+          setter_kn <- match setter_gr with
+          | ConstRef kn => ret kn
+          | _ => tmFail "Unexpected global_reference after unquoting"
+          end;;
 
-(* Setter provides a way to change a field given by a projection function, along
-with correctness conditions that require the projected field and only the
-projected field is modified. *)
-Class Setter {R T} (proj: R -> T) := set : (T -> T) -> R -> R.
-Arguments set {R T} proj {Setter}.
+          (* I could not find a way to specify the type of an unquoted constant,
+             so we always unquote as a cast *)
+          let body :=
+              tCast
+                (tConst setter_kn [])
+                Cast
+                (tApp
+                   <% @SetterFromGetter %>
+                   [tInd ind []; A; tConst getter_kn []]) in
 
-Class SetterWf {R T} (proj: R -> T) :=
-  { set_wf :> Setter proj;
-    set_get: forall v r, proj (set proj v r) = v (proj r);
-    set_eq: forall r, set proj (fun x => x) r = r; }.
+          let setter_from_getter_id := "setter_from_getter_" ^ ind_name oib ^ "_" ^ id in
+          tmMkDefinition setter_from_getter_id body;;
 
-Arguments set_wf {R T} proj {SetterWf}.
-
-Local Ltac SetterInstance_t :=
-  match goal with
-  | |- @Setter ?T _ ?A => get_setter T A
-  end.
-
-Local Ltac SetterWfInstance_t :=
-  match goal with
-  | |- @SetterWf ?T _ ?A =>
-    unshelve notypeclasses refine (Build_SetterWf _ _ _);
-    [ get_setter T A |
-      let r := fresh in
-      intros ? r; destruct r |
-      let r := fresh in
-      intros r; destruct r ];
-    intros; reflexivity
-  end.
-
-Hint Extern 1 (Setter _) => SetterInstance_t : typeclass_instances.
-Hint Extern 1 (SetterWf _) => SetterWfInstance_t : typeclass_instances.
+          tmLocate1 setter_from_getter_id >>= tmExistingInstance
+        | nAnon => ret tt
+        end;;
+        create_setters B (S idx)
+      | tLetIn na a A B => create_setters B idx
+      | _  => ret tt
+      end in
+  create_setters ctor 0.
 
 Module RecordSetNotations.
+  Declare Scope record_set.
   Delimit Scope record_set with rs.
   Open Scope rs.
-  Notation "x <| proj  :=  v |>" := (set proj (constructor v) x)
-                                    (at level 12, left associativity) : record_set.
-  Notation "x <| proj  ::=  f |>" := (set proj f x)
+  Notation "x <| proj  ::=  f |>" := ((_ : SetterFromGetter proj) f x)
                                      (at level 12, f at next level, left associativity) : record_set.
-  Notation "x <| proj1 ; proj2 ; .. ; projn := v |>" :=
-    (set proj1 (set proj2 .. (set projn (constructor v)) ..) x)
-    (at level 12, left associativity).
+  Notation "x <| proj  :=  v |>" := ((_ : SetterFromGetter proj) (fun _ => v) x)
+                                    (at level 12, left associativity) : record_set.
   Notation "x <| proj1 ; proj2 ; .. ; projn ::= f |>" :=
-    (set proj1 (set proj2 .. (set projn f) ..) x)
+    ((_ : SetterFromGetter proj1)
+       ((_ : SetterFromGetter proj2) .. ((_ : SetterFromGetter projn) f) ..) x)
+    (at level 12, left associativity).
+  Notation "x <| proj1 ; proj2 ; .. ; projn := v |>" :=
+    ((_ : SetterFromGetter proj1)
+       ((_ : SetterFromGetter proj2) .. ((_ : SetterFromGetter projn) (fun _ => v)) ..) x)
     (at level 12, left associativity).
 End RecordSetNotations.
