execution/examples/FA2Token.v
@@ -74,12 +74,9 @@ Record Setup :=
     transfer_hook_addr_       : option Address;
   }.
 
-Instance token_ledger_settable : Settable _ :=
-  settable! build_token_ledger <fungible; balances>.
-Instance state_settable : Settable _ :=
-  settable! build_state <fa2_owner; assets; operators; permission_policy; tokens; transfer_hook_addr>.
-Instance setup_settable : Settable _ :=
-  settable! build_setup <setup_total_supply; setup_tokens; initial_permission_policy; transfer_hook_addr_>.
+MetaCoq Run (make_setters TokenLedger).
+MetaCoq Run (make_setters State).
+MetaCoq Run (make_setters Setup).
 
 Section Serialization.
 
